vector

src/Init/Data/Vector/Basic.lean
@@ -319,7 +319,7 @@ This will perform the update destructively provided that the vector has a refere
 @[inline] def range (n : Nat) : Vector Nat n := ⟨Array.range n, by simp⟩
 
 /-- The vector `#v[start, start + step, start + 2 * step, ..., start + (size - 1) * step]`. -/
-@[inline] def range' (start size step : Nat) : Vector Nat size :=
+@[inline] def range' (start size : Nat) (step : Nat := 1) : Vector Nat size :=
   ⟨Array.range' start size step, by simp⟩
 
 /--
